code/rsapss/Hacl.RSAPSS.fst
@@ -1,16 +1,5 @@
 module Hacl.RSAPSS
 
-open FStar.HyperStack
-open FStar.HyperStack.ST
-open FStar.Mul
-
-open Lib.IntTypes
-open Lib.Buffer
-
-open Hacl.Bignum.Definitions
-open Hacl.Impl.MGF
-
-module ST = FStar.HyperStack.ST
 module S = Spec.RSAPSS
 module Hash = Spec.Agile.Hash
 
